examples/dsls/core/Refl.Typing.fsti
@@ -37,7 +37,23 @@ val pack_inspect_comp (t:R.comp)
 val inspect_pack_comp (t:R.comp_view)
   : Lemma (ensures (R.inspect_comp (R.pack_comp t) == t))
           [SMTPat (R.inspect_comp (R.pack_comp t))]
-  
+
+val pack_inspect_fv (fv:R.fv)
+  : Lemma (ensures R.pack_fv (R.inspect_fv fv) == fv)
+          [SMTPat (R.pack_fv (R.inspect_fv fv))]
+
+val inspect_pack_fv (nm:R.name)
+  : Lemma (ensures R.inspect_fv (R.pack_fv nm) == nm)
+          [SMTPat (R.inspect_fv (R.pack_fv nm))]
+
+val pack_inspect_universe (u:R.universe)
+  : Lemma (ensures R.pack_universe (R.inspect_universe u) == u)
+          [SMTPat (R.pack_universe (R.inspect_universe u))]
+
+val inspect_pack_universe (u:R.universe_view)
+  : Lemma (ensures R.inspect_universe (R.pack_universe u) == u)
+          [SMTPat (R.inspect_universe (R.pack_universe u))]
+
 val lookup_bvar (e:env) (x:int) : option term
 
 val lookup_fvar_uinst (e:R.env) (x:R.fv) (us:list R.universe) : option R.term
